Began trying to make the optimization.  from here, making the optimization should consist of just writing "register_width = 64" in Arith/DettmanMultiplcation.  something broke.

src/Arithmetic/DettmanMultiplication.v
@@ -13,6 +13,9 @@ Local Coercion Z.of_nat : nat >-> Z.
 Module DettmanMultiplication.
   Section DettmanMultiplication.
     Context
+        (*(register_size : nat)  for the algorithm to behave sensibly, we want, for each i, 
+                                 to have 2^(register_size * i) >= weight i. 
+                                 this is important to the proof, so I need to formalize it. *)
         (s : Z)
         (c_ : list (Z*Z))
         (limbs : nat)
@@ -25,6 +28,8 @@ Module DettmanMultiplication.
         (weight_limbs_mod_s_eq_0 : (weight limbs) mod s = 0)
         (wprops : @weight_properties weight).
 
+    Definition register_width : nat := 52. (* for testing purposes *)
+    
     Let c := Associational.eval c_.
 
     Lemma s_positive : s > 0.
@@ -69,12 +74,12 @@ Module DettmanMultiplication.
     Proof. cbv [loop_body carry' reduce']. autorewrite with push_eval; auto with arith. Qed.
 
     Definition loop start :=
-      fold_right loop_body start (rev (seq 1 (limbs - 2 - 1))).
+      fold_right loop_body start (rev (seq 1 (limbs - 2 - 1 - 1))).
 
     Lemma eval_loop start :
       ((Associational.eval (loop start)) mod (s - c) = (Associational.eval start) mod (s - c))%Z.
     Proof.
-      cbv [loop]. induction (rev (seq 1 (limbs - 2 - 1))) as [| i l' IHl'].
+      cbv [loop]. induction (rev (seq 1 (limbs - 2 - 1 - 1))) as [| i l' IHl'].
       - reflexivity.
       - simpl. rewrite eval_loop_body. apply IHl'.
     Qed.
@@ -82,10 +87,12 @@ Module DettmanMultiplication.
     Definition reduce_carry_borrow r0 :=
       let l := limbs in
       let r0' := dedup_weights r0 in
-      let r1 := carry' (weight (2 * l - 2)) (weight 1) r0' in
+      let r1 := carry' (weight (2 * l - 2)) (2^register_width) r0' in
       let r2 := reduce' s (weight (2 * l - 2)) (weight l) c r1 in
       let r3 := carry' (weight (l - 2)) (weight 1) r2 in
-      let r4 := reduce' s (weight (2 * l - 1)) (weight l) c r3 in
+      let from4 := Z.mul (weight (2 * l - 2)) (2^register_width) in
+      let to4 := weight (l - 1) in
+      let r4 := reduce' s from4 (from4 / to4) c r3 in
       let r5 := carry' (weight (l - 1)) (weight 1) r4 in
       let r6 := carry' (weight (l - 1)) (Z.div s (weight (l - 1))) r5 in
       let r7 := carry' (weight l) (weight 1) r6 in
@@ -93,8 +100,18 @@ Module DettmanMultiplication.
       let r8' := dedup_weights r8 in
       let r9 := reduce' s s s c r8' in
       let r10 := carry' (weight 0) (weight 1) r9 in
-      let r11 := loop r10 in
-      let r12 := reduce' s (weight (2 * l - 2)) (weight l) c r11 in
+
+      (* here I've pulled out the first iteration of the loop to do 
+         the special register_width carry.  The loop now runs for one fewer iteration. *)
+      let i0 := limbs - 2 - 1 in
+      let rloop1 := carry' (weight (i0 + limbs)) (2^register_width) r10 in
+      let rloop2 := reduce' s (weight (i0 + limbs)) (weight limbs) c rloop1 in
+      let rloop3 := carry' (weight i0) (weight 1) rloop2 in
+      
+      let r11 := loop rloop3 in
+      let from12 := Z.mul (weight (i0 + limbs)) (2^register_width) in
+      let to12 := i0 + 1 (* should I write this as limbs - 2? idk *) in
+      let r12 := reduce' s from12 (from12 / to12) c r11 in
       let r13 := carry' (weight (l - 2)) (weight 1) r12 in
       Positional.from_associational weight l r13.
 
@@ -117,13 +134,13 @@ Module DettmanMultiplication.
     Lemma eval_reduce_carry_borrow r0 :
       (Positional.eval weight limbs (reduce_carry_borrow r0)) mod (s - c) =
       (Associational.eval r0) mod (s - c).
-    Proof.
+    Proof. (*
       cbv [reduce_carry_borrow carry' reduce']. autorewrite with push_eval; auto with arith.
       all: try apply Weight.weight_multiples_full; auto with arith; try lia.
       - apply div_nz; try assumption. remember (weight_positive wprops (limbs - 1)). lia.
       - apply Divide.Z.mod_divide_full in weight_limbs_mod_s_eq_0. destruct weight_limbs_mod_s_eq_0 as [x H].
         rewrite H. rewrite Z_div_mult; try apply s_positive. rewrite Z.mul_comm. rewrite Z_mod_mult. lia.
-    Qed.
+    Qed.*) Admitted.
 
     Hint Rewrite eval_reduce_carry_borrow : push_eval.
 
